thy/PointerMapImpl.thy
@@ -14,8 +14,7 @@ begin
   definition is_pointermap_impl :: "('a::{hashable,heap}) pointermap \<Rightarrow> 'a pointermap_impl \<Rightarrow> assn" where
     "is_pointermap_impl b bi \<equiv> 
       is_array_list (entries b) (entriesi bi) 
-    * is_hashmap (getentry b) (getentryi bi)
-    * \<up>(pointermap_sane b)"
+    * is_hashmap (getentry b) (getentryi bi)"
 
   lemma is_pointermap_impl_prec: "precise is_pointermap_impl"
   	unfolding is_pointermap_impl_def[abs_def]
@@ -33,9 +32,6 @@ begin
 	apply blast
   done
 
-  lemma is_pi_sane_subst: "is_pointermap_impl b bi = \<up>(pointermap_sane b) * is_pointermap_impl b bi"
-    by (sep_auto simp: is_pointermap_impl_def)
-
   definition pointermap_empty where
     "pointermap_empty \<equiv> do {
       hm \<leftarrow> hm_new;
@@ -44,13 +40,14 @@ begin
     }"
 
   lemma [sep_heap_rules]: "< emp > pointermap_empty <is_pointermap_impl empty_pointermap>\<^sub>t"
-    unfolding is_pointermap_impl_def apply simp
+    unfolding is_pointermap_impl_def
     by (sep_auto simp: pointermap_empty_def empty_pointermap_def)
 
   definition pm_pthi where
     "pm_pthi m p \<equiv> arl_nth (entriesi m) p"
 
-  lemma [sep_heap_rules]: "pointermap_p_valid p m \<Longrightarrow> < is_pointermap_impl m mi > pm_pthi mi p <\<lambda>ai. is_pointermap_impl m mi * \<up>(ai = pm_pth m p)>"
+  lemma [sep_heap_rules]: "pointermap_sane m \<Longrightarrow> pointermap_p_valid p m \<Longrightarrow>
+  	< is_pointermap_impl m mi > pm_pthi mi p <\<lambda>ai. is_pointermap_impl m mi * \<up>(ai = pm_pth m p)>"
     by (sep_auto simp: pm_pthi_def pm_pth_def is_pointermap_impl_def pointermap_p_valid_def)
 
   definition pointermap_getmki where
@@ -69,10 +66,9 @@ begin
     }"
   
   lemmas pointermap_getmki_defs = pointermap_getmki_def pointermap_getmk_def pointermap_insert_def is_pointermap_impl_def
-  lemma [sep_heap_rules]: "pointermap_getmk a m = (p,u) \<Longrightarrow> 
-    < is_pointermap_impl m mi > pointermap_getmki a mi <\<lambda>(pi,ui). is_pointermap_impl u ui * \<up>(pi = p \<and> pointermap_p_valid p u)>\<^sub>t"
-    apply (subst is_pi_sane_subst; clarsimp)
-    apply (frule (1) pointermap_sane_getmkD)
+  lemma [sep_heap_rules]: "pointermap_sane m \<Longrightarrow> pointermap_getmk a m = (p,u) \<Longrightarrow> 
+    < is_pointermap_impl m mi > pointermap_getmki a mi 
+    <\<lambda>(pi,ui). is_pointermap_impl u ui * \<up>(pi = p)>\<^sub>t"
     apply(cases "getentry m a")
     apply(unfold pointermap_getmki_def)
     apply(unfold return_bind)
